Implements dec_ac and do some cleanup on other theories.

AC_equality.thy
@@ -4,8 +4,10 @@ imports Main "First_Order_Terms.Term" "Syntax"
 
 begin
 
-(*
+context signature
+begin
 
+(*
 Inductive definition of the relation =AC.
 
                       \<forall>i. t_i  =AC s_i   label f \<noteq> AC
@@ -32,14 +34,14 @@ espirito de porco?
 
 *)
 
-inductive eq_ac:: \<open>('v, 'f) term \<Rightarrow> ('v, 'f) term \<Rightarrow> bool\<close> where
+inductive eq_ac:: \<open>('f, 'v) term \<Rightarrow> ('f, 'v) term \<Rightarrow> bool\<close> where
   ac_refl: \<open>eq_ac t t\<close> |
   
   nac_fun: \<open> \<lbrakk>
           label f \<noteq> AC ;
           length ts > 0 ;
           length ts = length gs ;
-          i < length ts \<Longrightarrow> ts!i = gs!i
+          i < length ts \<Longrightarrow> eq_ac (ts!i) (gs!i)
           \<rbrakk> \<Longrightarrow> eq_ac (Fun f ts) (Fun f gs)\<close> |
 
   ac_fun: \<open>\<lbrakk>
@@ -51,6 +53,31 @@ inductive eq_ac:: \<open>('v, 'f) term \<Rightarrow> ('v, 'f) term \<Rightarrow>
             eq_ac (Fun f (remove1 (ts!1) ts)) (Fun f (remove1 (ts!i) ts))
           )
           \<rbrakk> \<Longrightarrow> eq_ac (Fun f ts) (Fun f gs)\<close>
+
+(* 
+
+  [x ; y ; z] = [y ; w ; x] \<Rightarrow> \<exists>j. x =AC rs!j, take j = 2 
+                            \<Longrightarrow> x =AC x \<and> [y ; z] = [y ; w]
+                            \<Longrightarrow> x =AC x \<and> y =AC y \<and> [z] = [w]
+                            \<Longrightarrow> False
+
+E = { x + y = y + x ; (x + y) + z = x + (y + z) }
+
+ \<approx>_E
+
+  T(\<Sigma>,X) / \<approx>E (this is an intial algebra)
+
+  Soundness for my unification:
+
+  if unif_ac(s,t) = \<sigma>, then s \<cdot> \<sigma> =AC t \<cdot> \<sigma> (syntactic soundness)
+  
+  s =AC t iff s \<approx>_AC t (algebraic soundness)
+
+  can i conclude:
+  
+  unif_ac(s,t) = \<sigma> \<Longrightarrow> s \<sigma> \<approx>_AC t \<sigma>
+*)
+
 
 text \<open> Next, we have to prove that this inductive relation is indeed an equivalent relation. \<close>
 
@@ -66,7 +93,14 @@ lemma ac_eq_trans: \<open>eq_ac s t \<and> eq_ac t u \<Longrightarrow> eq_ac s u
 
 
 lemma ac_eq_subst: \<open>eq_ac s t \<Longrightarrow> eq_ac (s \<cdot> \<sigma>) (t \<cdot> \<sigma>)\<close>
-  sorry
+proof (induction s)
+  case (Var x)
+  then show ?case sorry
+next
+  case (Fun f ts)
+  then show ?case sorry
+qed
+ 
 
 (* Question 1: is this really closure for \<Sigma>-operations when the arguments are lists?
   I'm thinking I have to say something like: \<forall> t \<in> set ts. ... 
@@ -74,3 +108,53 @@ lemma ac_eq_subst: \<open>eq_ac s t \<Longrightarrow> eq_ac (s \<cdot> \<sigma>)
 *)
 lemma ac_eq_fun: \<open>eq_ac s t \<Longrightarrow> eq_ac (Fun f [s]) (Fun f [t])\<close>
   sorry
+
+section \<open>Decidability of AC equality \<close>
+
+text \<open>The purpose of this function is to then algorithimically decide the relation above.
+
+We implement the deduction rules above as follows by destruction on their structure:
+1. Two Vars are equal if they underlying names are equal.
+  - It is sound because we can never show x = y with x \<noteq> y using reflexivity.
+2. Compare whenever we have a variable and a function, those are all false.
+
+3. We compare when the two terms are of the shape: (Fun f ts) (Fun g gs)
+
+  
+
+\<close>
+
+
+function dec_ac :: \<open>('f, 'v) term \<Rightarrow> ('f, 'v) term \<Rightarrow> bool\<close> where
+  \<open>dec_ac (Var x) (Var y) = (x = y)\<close> |
+  \<open>dec_ac (Var _) (Fun _ _) = False\<close> |
+  \<open>dec_ac (Fun _ _) (Var _) = False\<close> |
+  \<open>dec_ac (Fun f ts) (Fun g gs) = (
+    if (f = g) \<and> (length ts = length gs) then
+      (if length ts = 0 then
+        True
+      else
+        (case label f of
+          AC \<Rightarrow> (
+            let t0 = hd ts in
+            let eq_exists = find (\<lambda> sj. dec_ac t0 sj) gs  in
+            (case eq_exists of
+              None \<Rightarrow> False |
+              Some sj \<Rightarrow> dec_ac (Fun f (remove1 t0 ts)) (Fun f (remove1 sj gs)))
+          )|
+          _ \<Rightarrow> foldl (\<and>) True (map (\<lambda> (x,y). dec_ac x y) (zip ts gs))
+        )
+      )
+    else
+      False
+  )\<close>
+  by pat_completeness auto
+
+value "dec_ac (Var 0) (Fun f [Var 0])" (* I don't know why this doesn't compute since this case doesnt'depend on how label is defined... *)
+
+end
+
+print_locale! signature
+
+
+end
